2.5.3. Covariance and Variance of Sums of Random Variables

The covariance of any two random variables *X* and *Y*, denoted by Cov(X, Y), is defined by

$$Cov(X, Y) = E[(X - E[X])(Y - E[Y])]$$

= $E[XY - YE[X] - XE[Y] + E[X]E[Y]]$
= $E[XY] - E[Y]E[X] - E[X]E[Y] + E[X]E[Y]$
= $E[XY] - E[X]E[Y]$

Note that if *X* and *Y* are independent, then by Proposition 2.3 it follows that Cov(X, Y) = 0.

Let us consider now the special case where X and Y are indicator variables for whether or not the events A and B occur. That is, for events A and B, define

$$X = \begin{cases} 1, & \text{if } A \text{ occurs} \\ 0, & \text{otherwise,} \end{cases} \quad Y = \begin{cases} 1, & \text{if } B \text{ occurs} \\ 0, & \text{otherwise} \end{cases}$$

Then,

$$Cov(X, Y) = E[XY] - E[X]E[Y]$$

and, because XY will equal 1 or 0 depending on whether or not both X and Y equal 1, we see that

$$Cov(X, Y) = P\{X = 1, Y = 1\} - P\{X = 1\}P\{Y = 1\}$$

From this we see that

$$\begin{split} \operatorname{Cov}(X,Y) > 0 &\Leftrightarrow P\{X=1,Y=1\} > P\{X=1\}P\{Y=1\} \\ &\Leftrightarrow \frac{P\{X=1,Y=1\}}{P\{X=1\}} > P\{Y=1\} \\ &\Leftrightarrow P\{Y=1|X=1\} > P\{Y=1\} \end{split}$$

That is, the covariance of X and Y is positive if the outcome X = 1 makes it more likely that Y = 1 (which, as is easily seen by symmetry, also implies the reverse).

In general it can be shown that a positive value of Cov(X, Y) is an indication that Y tends to increase as X does, whereas a negative value indicates that Y tends to decrease as X increases.

The following are important properties of covariance.

Properties of Covariance

For any random variables X, Y, Z and constant c,

- 1. $\operatorname{Cov}(X, X) = \operatorname{Var}(X)$,
- 2. $\operatorname{Cov}(X, Y) = \operatorname{Cov}(Y, X),$
- 3. $\operatorname{Cov}(cX, Y) = c\operatorname{Cov}(X, Y),$
- 4. $\operatorname{Cov}(X, Y + Z) = \operatorname{Cov}(X, Y) + \operatorname{Cov}(X, Z).$

Whereas the first three properties are immediate, the final one is easily proven as follows:

$$Cov(X, Y + Z) = E[X(Y + Z)] - E[X]E[Y + Z]$$
$$= E[XY] - E[X]E[Y] + E[XZ] - E[X]E[Z]$$
$$= Cov(X, Y) + Cov(X, Z)$$

The fourth property listed easily generalizes to give the following result:

$$\operatorname{Cov}\left(\sum_{i=1}^{n} X_{i}, \sum_{j=1}^{m} Y_{j}\right) = \sum_{i=1}^{n} \sum_{j=1}^{m} \operatorname{Cov}(X_{i}, Y_{j})$$
(2.15)

A useful expression for the variance of the sum of random variables can be obtained from Equation (2.15) as follows:

$$\operatorname{Var}\left(\sum_{i=1}^{n} X_{i}\right) = \operatorname{Cov}\left(\sum_{i=1}^{n} X_{i}, \sum_{j=1}^{n} X_{j}\right)$$
$$= \sum_{i=1}^{n} \sum_{j=1}^{n} \operatorname{Cov}(X_{i}, X_{j})$$
$$= \sum_{i=1}^{n} \operatorname{Cov}(X_{i}, X_{i}) + \sum_{i=1}^{n} \sum_{j \neq i} \operatorname{Cov}(X_{i}, X_{j})$$
$$= \sum_{i=1}^{n} \operatorname{Var}(X_{i}) + 2\sum_{i=1}^{n} \sum_{j < i} \operatorname{Cov}(X_{i}, X_{j}) \qquad (2.16)$$

If X_i , i = 1, ..., n are independent random variables, then Equation (2.16) reduces to

$$\operatorname{Var}\left(\sum_{i=1}^{n} X_{i}\right) = \sum_{i=1}^{n} \operatorname{Var}(X_{i})$$

Definition 2.1 If $X_1, ..., X_n$ are independent and identically distributed, then the random variable $\bar{X} = \sum_{i=1}^{n} X_i/n$ is called the *sample mean*.

The following proposition shows that the covariance between the sample mean and a deviation from that sample mean is zero. It will be needed in Section 2.6.1.

Proposition 2.4 Suppose that X_1, \ldots, X_n are independent and identically distributed with expected value μ and variance σ^2 . Then,

- (a) $E[\bar{X}] = \mu$.
- (b) $\operatorname{Var}(\bar{X}) = \sigma^2/n$.
- (c) $\operatorname{Cov}(\bar{X}, X_i \bar{X}) = 0, \ i = 1, \dots, n.$

Proof Parts (a) and (b) are easily established as follows:

$$E[\bar{X}] = \frac{1}{n} \sum_{i=1}^{m} E[X_i] = \mu,$$

$$\operatorname{Var}(\bar{X}) = \left(\frac{1}{n}\right)^2 \operatorname{Var}\left(\sum_{i=1}^{n} X_i\right) = \left(\frac{1}{n}\right)^2 \sum_{i=1}^{n} \operatorname{Var}(X_i) = \frac{\sigma^2}{n}$$

To establish part (c) we reason as follows:

$$\operatorname{Cov}(\bar{X}, X_i - \bar{X}) = \operatorname{Cov}(\bar{X}, X_i) - \operatorname{Cov}(\bar{X}, \bar{X})$$
$$= \frac{1}{n} \operatorname{Cov}\left(X_i + \sum_{j \neq i} X_j, X_i\right) - \operatorname{Var}(\bar{X})$$
$$= \frac{1}{n} \operatorname{Cov}(X_i, X_i) + \frac{1}{n} \operatorname{Cov}\left(\sum_{j \neq i} X_j, X_i\right) - \frac{\sigma^2}{n}$$
$$= \frac{\sigma^2}{n} - \frac{\sigma^2}{n} = 0$$

where the final equality used the fact that X_i and $\sum_{j \neq i} X_j$ are independent and thus have covariance 0.

Equation (2.16) is often useful when computing variances.

Example 2.33 (Variance of a Binomial Random Variable) Compute the variance of a binomial random variable X with parameters n and p.